fv/lean/Ragu/Instances/Point/Double.lean
@@ -5,74 +5,106 @@ namespace Ragu.Instances.Point.Double
 open Core.Primes
 
 @[reducible]
-def CircuitField := F Core.Primes.p
+def p := Core.Primes.p
 
-def Inputs := ProvableVector field 2
+@[reducible]
+def inputLen := 2
 
--- Point doubling instance:
+@[reducible]
+def outputLen := 2
+
 set_option linter.unusedVariables false in
-def exported_operations (input_var : Var Inputs CircuitField) : Operations CircuitField := [
+def exportedOperations (input_var : Var (ProvableVector field inputLen) (F p)) : Operations (F p) := [
   Operation.witness 3 (fun _env => default),
-  Operation.assert ((((var 0) * (var 1)) + ((0x40000000000000000000000000000000224698fc094cf91b992d30ed00000000 : Expression CircuitField) * (var 2)))),
-  Operation.assert (((var 0) + ((0x40000000000000000000000000000000224698fc094cf91b992d30ed00000000 : Expression CircuitField) * (input_var.get 0)))),
-  Operation.assert (((var 1) + ((0x40000000000000000000000000000000224698fc094cf91b992d30ed00000000 : Expression CircuitField) * (input_var.get 0)))),
+  Operation.assert ((((var 0) * (var 1)) + ((0x40000000000000000000000000000000224698fc094cf91b992d30ed00000000 : Expression (F p)) * (var 2)))),
+  Operation.assert (((var 0) + ((0x40000000000000000000000000000000224698fc094cf91b992d30ed00000000 : Expression (F p)) * (input_var.get 0)))),
+  Operation.assert (((var 1) + ((0x40000000000000000000000000000000224698fc094cf91b992d30ed00000000 : Expression (F p)) * (input_var.get 0)))),
   Operation.witness 3 (fun _env => default),
-  Operation.assert ((((var 3) * (var 4)) + ((0x40000000000000000000000000000000224698fc094cf91b992d30ed00000000 : Expression CircuitField) * (var 5)))),
-  Operation.assert ((((0x0000000000000000000000000000000000000000000000000000000000000003 : Expression CircuitField) * (var 2)) + ((0x40000000000000000000000000000000224698fc094cf91b992d30ed00000000 : Expression CircuitField) * (var 5)))),
-  Operation.assert ((((input_var.get 1) + (input_var.get 1)) + ((0x40000000000000000000000000000000224698fc094cf91b992d30ed00000000 : Expression CircuitField) * (var 4)))),
+  Operation.assert ((((var 3) * (var 4)) + ((0x40000000000000000000000000000000224698fc094cf91b992d30ed00000000 : Expression (F p)) * (var 5)))),
+  Operation.assert ((((0x0000000000000000000000000000000000000000000000000000000000000003 : Expression (F p)) * (var 2)) + ((0x40000000000000000000000000000000224698fc094cf91b992d30ed00000000 : Expression (F p)) * (var 5)))),
+  Operation.assert ((((input_var.get 1) + (input_var.get 1)) + ((0x40000000000000000000000000000000224698fc094cf91b992d30ed00000000 : Expression (F p)) * (var 4)))),
   Operation.witness 3 (fun _env => default),
-  Operation.assert ((((var 6) * (var 7)) + ((0x40000000000000000000000000000000224698fc094cf91b992d30ed00000000 : Expression CircuitField) * (var 8)))),
-  Operation.assert (((var 6) + ((0x40000000000000000000000000000000224698fc094cf91b992d30ed00000000 : Expression CircuitField) * (var 3)))),
-  Operation.assert (((var 7) + ((0x40000000000000000000000000000000224698fc094cf91b992d30ed00000000 : Expression CircuitField) * (var 3)))),
+  Operation.assert ((((var 6) * (var 7)) + ((0x40000000000000000000000000000000224698fc094cf91b992d30ed00000000 : Expression (F p)) * (var 8)))),
+  Operation.assert (((var 6) + ((0x40000000000000000000000000000000224698fc094cf91b992d30ed00000000 : Expression (F p)) * (var 3)))),
+  Operation.assert (((var 7) + ((0x40000000000000000000000000000000224698fc094cf91b992d30ed00000000 : Expression (F p)) * (var 3)))),
   Operation.witness 3 (fun _env => default),
-  Operation.assert ((((var 9) * (var 10)) + ((0x40000000000000000000000000000000224698fc094cf91b992d30ed00000000 : Expression CircuitField) * (var 11)))),
-  Operation.assert (((var 9) + ((0x40000000000000000000000000000000224698fc094cf91b992d30ed00000000 : Expression CircuitField) * (var 3)))),
-  Operation.assert (((var 10) + ((0x40000000000000000000000000000000224698fc094cf91b992d30ed00000000 : Expression CircuitField) * ((input_var.get 0) + ((0x40000000000000000000000000000000224698fc094cf91b992d30ed00000000 : Expression CircuitField) * ((var 8) + ((0x40000000000000000000000000000000224698fc094cf91b992d30ed00000000 : Expression CircuitField) * ((input_var.get 0) + (input_var.get 0))))))))),
+  Operation.assert ((((var 9) * (var 10)) + ((0x40000000000000000000000000000000224698fc094cf91b992d30ed00000000 : Expression (F p)) * (var 11)))),
+  Operation.assert (((var 9) + ((0x40000000000000000000000000000000224698fc094cf91b992d30ed00000000 : Expression (F p)) * (var 3)))),
+  Operation.assert (((var 10) + ((0x40000000000000000000000000000000224698fc094cf91b992d30ed00000000 : Expression (F p)) * ((input_var.get 0) + ((0x40000000000000000000000000000000224698fc094cf91b992d30ed00000000 : Expression (F p)) * ((var 8) + ((0x40000000000000000000000000000000224698fc094cf91b992d30ed00000000 : Expression (F p)) * ((input_var.get 0) + (input_var.get 0))))))))),
 ]
 
 set_option linter.unusedVariables false in
 @[reducible]
-def exported_output (input_var : Var Inputs CircuitField) : Vector (Expression CircuitField) 2 := #v[
-  ((var 8) + ((0x40000000000000000000000000000000224698fc094cf91b992d30ed00000000 : Expression CircuitField) * ((input_var.get 0) + (input_var.get 0)))),
-  ((var 11) + ((0x40000000000000000000000000000000224698fc094cf91b992d30ed00000000 : Expression CircuitField) * (input_var.get 1)))
+def exportedOutput (input_var : Var (ProvableVector field inputLen) (F p)) : Vector (Expression (F p)) 2 := #v[
+  ((var 8) + ((0x40000000000000000000000000000000224698fc094cf91b992d30ed00000000 : Expression (F p)) * ((input_var.get 0) + (input_var.get 0)))),
+  ((var 11) + ((0x40000000000000000000000000000000224698fc094cf91b992d30ed00000000 : Expression (F p)) * (input_var.get 1)))
 ]
 
-def circuit := Circuits.Point.Double.circuit Circuits.Point.Spec.EpAffineParams (p:=Core.Primes.p)
-
-def deserializeInput (input : Var Inputs CircuitField) : Var Circuits.Point.Spec.Point CircuitField :=
+def deserializeInput (input : Var (ProvableVector field inputLen) (F p)) : Var Circuits.Point.Spec.Point (F p) :=
   {
     x := input.get 0,
     y := input.get 1
   }
 
-def serializeOutput (output: Var Circuits.Point.Spec.Point CircuitField) : Vector (Expression CircuitField) 2 :=
+def serializeOutput (output: Var Circuits.Point.Spec.Point (F p)) : Vector (Expression (F p)) 2 :=
   #v[
     output.x,
     output.y
   ]
 
-theorem same_circuit (input : Var Inputs CircuitField):
-    ((circuit (deserializeInput input)).operations 0).toFlat = (exported_operations input).toFlat := by
-  simp [Operations.toFlat, circuit_norm, FormalCircuit.toSubcircuit,
-    circuit, deserializeInput, exported_operations,
-    Circuits.Point.Double.circuit, Circuits.Point.Double.elaborated, Circuits.Point.Double.main,
-    Circuits.Core.AllocMul.circuit, Circuits.Core.AllocMul.elaborated, Circuits.Core.AllocMul.main,
-    Circuits.Element.Square.circuit, Circuits.Element.Square.elaborated, Circuits.Element.Square.main,
-    Circuits.Element.DivNonzero.circuit, Circuits.Element.DivNonzero.elaborated, Circuits.Element.DivNonzero.main,
-    Circuits.Element.Mul.circuit, Circuits.Element.Mul.elaborated, Circuits.Element.Mul.main]
-  repeat (constructor; rfl)
-  constructor
+def formal_instance : Core.Statements.FormalInstance where
+  p
+  inputLen
+  outputLen
+  exportedOperations
+  exportedOutput
 
-theorem same_output (input : Var Inputs CircuitField) :
-    ((deserializeInput input) |> circuit |>.output 0 |> serializeOutput) = exported_output input:= by
-  simp [circuit_norm, FormalCircuit.toSubcircuit,
-    circuit, deserializeInput, serializeOutput,
-    Circuits.Point.Double.circuit, Circuits.Point.Double.elaborated, Circuits.Point.Double.main,
-    Circuits.Core.AllocMul.circuit, Circuits.Core.AllocMul.elaborated, Circuits.Core.AllocMul.main,
-    Circuits.Element.Square.circuit, Circuits.Element.Square.elaborated, Circuits.Element.Square.main,
-    Circuits.Element.DivNonzero.circuit, Circuits.Element.DivNonzero.elaborated, Circuits.Element.DivNonzero.main,
-    Circuits.Element.Mul.circuit, Circuits.Element.Mul.elaborated, Circuits.Element.Mul.main]
-  constructor <;> rfl
+  Input := Circuits.Point.Spec.Point
+  Output := Circuits.Point.Spec.Point
 
+  deserializeInput
+  serializeOutput
+
+  Assumptions input :=
+    input.isOnCurve Circuits.Point.Spec.EpAffineParams ∧
+    Circuits.Point.Spec.EpAffineParams.noOrderTwoPoints
+
+  Spec input output :=
+    (match input.double with
+    | none => False -- this case never happens
+    | some double => output = double)
+    ∧
+    output.isOnCurve Circuits.Point.Spec.EpAffineParams
+
+
+  reimplementation := Circuits.Point.Double.circuit Circuits.Point.Spec.EpAffineParams
+
+  same_circuit := by
+    intro input
+    simp [Operations.toFlat, circuit_norm, FormalCircuit.toSubcircuit,
+      deserializeInput, exportedOperations,
+      Circuits.Point.Double.circuit, Circuits.Point.Double.elaborated, Circuits.Point.Double.main,
+      Circuits.Core.AllocMul.circuit, Circuits.Core.AllocMul.elaborated, Circuits.Core.AllocMul.main,
+      Circuits.Element.Square.circuit, Circuits.Element.Square.elaborated, Circuits.Element.Square.main,
+      Circuits.Element.DivNonzero.circuit, Circuits.Element.DivNonzero.elaborated, Circuits.Element.DivNonzero.main,
+      Circuits.Element.Mul.circuit, Circuits.Element.Mul.elaborated, Circuits.Element.Mul.main]
+    repeat (constructor; rfl)
+    constructor
+  same_output := by
+    intro input;
+    simp [circuit_norm, FormalCircuit.toSubcircuit,
+      deserializeInput, serializeOutput,
+      Circuits.Point.Double.circuit, Circuits.Point.Double.elaborated, Circuits.Point.Double.main,
+      Circuits.Core.AllocMul.circuit, Circuits.Core.AllocMul.elaborated, Circuits.Core.AllocMul.main,
+      Circuits.Element.Square.circuit, Circuits.Element.Square.elaborated, Circuits.Element.Square.main,
+      Circuits.Element.DivNonzero.circuit, Circuits.Element.DivNonzero.elaborated, Circuits.Element.DivNonzero.main,
+      Circuits.Element.Mul.circuit, Circuits.Element.Mul.elaborated, Circuits.Element.Mul.main]
+    constructor <;> rfl
+  same_spec := by
+    intro input output;
+    simp [Circuits.Point.Double.circuit, Circuits.Point.Double.Spec]
+    intro h1
+    aesop
+  same_assumptions := by intro input; rfl
 
 end Ragu.Instances.Point.Double
